Add non-recursive let and refactor Arrow code

cava/arrow-lib/Kappa.v
@@ -1,56 +1,201 @@
+From Coq Require Import List Peano_dec.
 From Arrow Require Import Category Arrow.
 
+Import ListNotations.
+
+Set Implicit Arguments.
+Set Asymmetric Patterns.
+
 Section Arrow.
-  Context `{A: ArrowSTKC}.
+  Context `{arrow: Arrow}.
+
+  Notation object_pair := (object * object)%type.
+  Definition natvar : object -> object -> Type := fun _ _ => nat.
+  Definition unitvar : object -> object -> Type := fun _ _ => unit.
 
   Section Vars.
     Variable (var: object -> object -> Type).
 
-    Local Open Scope arrow_scope.
-    Local Open Scope category_scope.
-
     Inductive kappa : object -> object -> Type :=
     | Var : forall {x y},   var x y -> kappa x y
-    | Abs : forall x {y z}, (var u x -> kappa y z) -> kappa (x ** y) z
-    | App : forall {x y z}, kappa (x ** y) z -> kappa u x -> kappa y z
+    | Abs : forall {x y z}, (var u x -> kappa y z) -> kappa (product x y) z
+    | App : forall {x y z}, kappa (product x y) z -> kappa u x -> kappa y z
     | Comp: forall {x y z}, kappa y z -> kappa x y -> kappa x z
     | Morph : forall {x y}, morphism x y -> kappa x y
-    | LetRec : forall x {y z}, 
-        (var u x -> kappa u x)
-      -> (var u x -> kappa y z) 
-      -> kappa y z.
-
-    Inductive NoLetRecKappa: forall i o, kappa i o -> Prop :=
-    | NoLetRecVar: forall x y v, NoLetRecKappa x y (Var v)
-    | NoLetRecAbs: forall x y z f,
-      (forall (k: var u x), NoLetRecKappa y z (f k)) -> NoLetRecKappa (x**y) z (Abs _ f)
-    | NoLetRecApp: forall x y z f e,
-      NoLetRecKappa (x ** y) z f -> NoLetRecKappa u x e -> NoLetRecKappa y z (App f e)
-    | NoLetRecComp: forall x y z f g,
-      NoLetRecKappa y z f -> NoLetRecKappa x y g -> NoLetRecKappa x z (Comp f g)
-    | NoLetRecMorph : forall x y m, NoLetRecKappa x y (Morph m).
-
-    Section prop.
-      Variable (P: forall x y, morphism x y -> Prop).
-
-      Inductive MorphPropKappa: forall i o, kappa i o -> Prop :=
-      | MorphPropVar: forall x y v, MorphPropKappa x y (Var v)
-      | MorphPropAbs: forall x y z f, (forall (k: var u x), MorphPropKappa y z (f k)) -> MorphPropKappa (x**y) z (Abs _ f)
-      | MorphPropApp: forall x y z f e,
-        MorphPropKappa (x ** y) z f -> MorphPropKappa u x e -> MorphPropKappa y z (App f e)
-      | MorphPropComp: forall x y z f g,
-        MorphPropKappa y z f -> MorphPropKappa x y g -> MorphPropKappa x z (Comp f g)
-      | MorphPropMorph : forall x y m, P x y m -> MorphPropKappa x y (Morph m).
-    End prop.
-
+    | Let: forall {x y z}, kappa u x -> (var u x -> kappa y z) -> kappa y z
+    | LetRec : forall {x y z}, (var u x -> kappa u x) -> (var u x -> kappa y z) -> kappa y z.
   End Vars.
 
-  Definition Kappa i o := forall var, kappa var i o.
+  Fixpoint reverse_nth {A} (l: list A) (n: nat) {struct l}: option A := 
+    match l with
+    | [] => None
+    | x :: xs => 
+      match eq_nat_dec n (length xs) with
+      | left _ => Some x
+      | right Hneq => reverse_nth xs n
+      end
+    end.
 
+  Notation ok_lookup := (fun (l: list _) (n: nat) (ty: _) => reverse_nth l n = Some ty).
+
+  Fixpoint wf_phoas_context {i o}
+    (ctxt: list object)
+    (expr: kappa natvar i o) {struct expr}
+    : Prop :=
+    match expr with
+    | Var _ _ n  => ok_lookup ctxt n o
+    | Abs x _ _ f => wf_phoas_context (x :: ctxt) (f (length ctxt))
+    | App _ _ _ e1 e2 => wf_phoas_context ctxt e1 /\ wf_phoas_context ctxt e2 
+    | Comp _ _ _ e1 e2 => wf_phoas_context ctxt e1 /\ wf_phoas_context ctxt e2
+    | Morph _ _ _ => True
+    | Let x _ _ v f => wf_phoas_context (x :: ctxt) (f (length ctxt)) /\ wf_phoas_context ctxt v 
+    | LetRec x _ _ v f => wf_phoas_context (x :: ctxt) (v (length ctxt)) /\ wf_phoas_context (x :: ctxt) (f (length ctxt))
+    end.
+
+  Section ctxt.
+    Context {ctxt: list object}.
+  
+    Lemma wf_phoas_context_lax_abs: forall {x y z} f,
+      @wf_phoas_context (product x y) z ctxt (Abs f) -> @wf_phoas_context y z (x :: ctxt) (f (length ctxt)).
+    Proof. auto. Qed.
+
+    Hint Extern 10 => 
+      match goal with
+      | [H: wf_phoas_context (_ :: ?ctxt) (Var _ ?v) |- _] => 
+        unfold wf_phoas_context, reverse_nth in H;
+        destruct (PeanoNat.Nat.eq_dec v (length ctxt))
+      | [H: wf_phoas_context _ _ |- _] => inversion H
+      end : core.
+  
+    Lemma wf_phoas_context_lax_var: forall {x y a} v ,
+      wf_phoas_context (i:=x) (o:=y) (a :: ctxt) (Var _ v) -> wf_phoas_context ctxt (Var _ v) \/ v = length ctxt.
+    Proof. auto. Qed.
+  
+    Lemma wf_phoas_context_lax_compose1: forall {x y z} e1 e2,
+      @wf_phoas_context x z ctxt (Comp e2 e1) -> @wf_phoas_context x y ctxt e1.
+    Proof. auto. Qed.
+  
+    Lemma wf_phoas_context_lax_compose2: forall {x y z} e1 e2,
+      @wf_phoas_context x z ctxt (Comp e2 e1) -> @wf_phoas_context y z ctxt e2.
+    Proof. auto. Qed.
+  
+    Lemma wf_phoas_context_lax_app1: forall {x y z} f e,
+      wf_phoas_context ctxt (App f e) -> @wf_phoas_context (product x y) z ctxt f.
+    Proof. auto. Qed.
+  
+    Lemma wf_phoas_context_lax_app2: forall {x y z} f e,
+      @wf_phoas_context y z ctxt (App f e) -> @wf_phoas_context u x ctxt e.
+    Proof. auto. Qed.
+
+    Lemma wf_phoas_context_lax_let1: forall {x y z} v f,
+      @wf_phoas_context y z ctxt (Let v f)
+      -> @wf_phoas_context u x ctxt v.
+    Proof. auto. Qed.
+
+    Lemma wf_phoas_context_lax_let2: forall {x y z} v f,
+      @wf_phoas_context y z ctxt (Let (x:=x) v f)
+      -> @wf_phoas_context y z (x :: ctxt) (f (length ctxt)).
+    Proof. auto. Qed.
+  
+    Lemma wf_phoas_context_lax_letrec1: forall {x y z} v f,
+      @wf_phoas_context y z ctxt (LetRec v f)
+      -> @wf_phoas_context u x (x :: ctxt) (v (length ctxt)).
+    Proof. auto. Qed.
+  
+    Lemma wf_phoas_context_lax_letrec2: forall {x y z} v f,
+      @wf_phoas_context y z ctxt (LetRec (x:=x) v f)
+      -> @wf_phoas_context y z (x :: ctxt) (f (length ctxt)).
+    Proof. auto. Qed.
+  End ctxt.
+    
+
+  Fixpoint wf_phoas_context_elim {i o}
+    (ctxt: list object)
+    (expr: kappa natvar i o) {struct expr}
+    : Prop :=
+    match expr with
+    | Var _ _ n  => ok_lookup ctxt n o
+    | Abs x _ _ f => wf_phoas_context_elim (x :: ctxt) (f (length ctxt))
+    | App _ _ _ e1 e2 => forall (p: Prop),
+      (wf_phoas_context_elim ctxt e1 -> wf_phoas_context_elim ctxt e2 -> p) -> p
+    | Comp _ _ _ e1 e2 => forall (p: Prop),
+      (wf_phoas_context_elim ctxt e1 -> wf_phoas_context_elim ctxt e2 -> p) -> p
+    | Morph _ _ _ => True
+    | Let x _ _ v f => forall (p: Prop), 
+      (wf_phoas_context_elim ctxt v -> wf_phoas_context_elim (x :: ctxt) (f (length ctxt)) -> p) -> p
+    | LetRec x _ _ v f => forall (p: Prop),
+      (wf_phoas_context_elim (x :: ctxt) (v (length ctxt))
+      -> wf_phoas_context_elim (x :: ctxt) (f (length ctxt)) -> p) -> p
+    end.
+
+  Goal forall x, wf_phoas_context [] (Abs (x:=x) (y:=u) (z:=x) (fun x => Let (Var _ x) (fun y => Var _ y))).
+  Proof. cbn; auto. Qed.
+  Goal forall x, wf_phoas_context_elim [] (Abs (x:=x) (y:=u) (z:=x) (fun x => Let (Var _ x) (fun y => Var _ y))).
+  Proof. cbn; auto. Qed.
+
+  Lemma phoas_context_elim {i o} (expr: kappa natvar i o): forall (ctxt: list object),
+    wf_phoas_context_elim ctxt expr -> wf_phoas_context ctxt expr.
+  Proof.
+    induction expr; cbn [wf_phoas_context_elim] in *; 
+      simpl; intros;
+      try constructor;
+      try apply H;
+      try apply H0;
+      try apply H1;
+      auto.
+  Qed.
+
+  Lemma wf_let_is_wf_app_abs {x i o}
+    (v: kappa natvar u x)
+    (f: natvar u x -> kappa natvar i o)
+    : forall (ctxt: list object), wf_phoas_context ctxt (Let v f) -> wf_phoas_context ctxt (App (Abs f) v).
+  Proof. now cbn. Qed.
+  
+  Fixpoint no_letrec {i o} (e: kappa unitvar i o): bool :=
+    match e with 
+    | Var _ _ _ => true 
+    | Abs _ _ _ f => no_letrec (f tt)
+    | App _ _ _ f e => no_letrec f && no_letrec e 
+    | Comp _ _ _ e1 e2 => no_letrec e1 && no_letrec e2
+    | Morph _ _ _ => true
+    | Let _ _ _ v f => no_letrec v && no_letrec (f tt) 
+    | LetRec _ _ _ f1 f2 => false
+    end.
+
+  Fixpoint morph_prop {i o}
+    (P: forall x y, morphism x y -> Prop)
+    (e: kappa unitvar i o)
+    : Prop :=
+    match e with 
+    | Var _ _ _ => True 
+    | Abs _ _ _ f => morph_prop P (f tt)
+    | App _ _ _ f e => forall p: Prop, (morph_prop P f -> morph_prop P e -> p) -> p
+    | Comp _ _ _ e1 e2 => forall p: Prop, (morph_prop P e1 -> morph_prop P e2 -> p) -> p
+    | Morph _ _ m => P _ _ m
+    | Let _ _ _ v f => forall p: Prop, (morph_prop P v -> morph_prop P (f tt) -> p) -> p
+    | LetRec _ _ _ f1 f2 => forall p: Prop, (morph_prop P (f1 tt) -> morph_prop P (f2 tt) -> p) -> p
+    end.
+
+    Definition Kappa i o := forall var, kappa var i o.
 End Arrow.
 
-Hint Constructors NoLetRecKappa : core.
-Hint Extern 5 (NoLetRecKappa _ _ _ _) => apply NoLetRecAbs : core.
-Hint Constructors MorphPropKappa : core.
-Hint Extern 5 (MorphPropKappa _ _ _ _ _) => apply MorphPropAbs : core.
-Hint Extern 10 (MorphPropKappa _ _ _ _ _) => apply MorphPropComp : core.
+Ltac dispatch_wf_phoas_context := 
+  apply phoas_context_elim;
+  lazy -[reverse_nth];
+  repeat lazymatch goal with
+  | [ |- True ] => exact I
+  | [ |- forall p, (?H1 -> ?H2 -> p) -> p ] => 
+    let x := fresh in (let y := fresh in (
+      intros x y; apply y; clear x y
+    ))
+  end; 
+  repeat lazymatch goal with
+  | [ |- reverse_nth _ _ = Some _] => exact eq_refl
+  end. 
+
+Arguments Kappa.Var {_ _ _ _ _ var _ _}.
+Arguments Kappa.Abs {_ _ _ _ _ var _ _ _}.
+Arguments Kappa.App {_ _ _ _ _ var _ _ _}.
+Arguments Kappa.Comp {_ _ _ _ _ var _ _ _}.
+Arguments Kappa.Morph {_ _ _ _ _ var _ _}.
+Arguments Kappa.LetRec {_ _ _ _ _ var _ _ _}.
