cava/arrow-lib/Equiv.v
@@ -1,0 +1,67 @@
+From Coq Require Import List PeanoNat Arith.Peano_dec.
+From Arrow Require Import Category Arrow Kappa.
+
+Import ListNotations.
+
+Set Implicit Arguments.
+Set Asymmetric Patterns.
+
+Section Arrow.
+  Context `{arrow: Arrow}.
+
+  Section Equivalence.
+    Inductive obj_tup : Type := obj_pair : object -> object -> obj_tup.
+    Variables var1 var2 : object -> object -> Type.
+
+    Definition vars := existT (fun '(obj_pair x y) => (var1 x y * var2 x y)%type).
+    Definition ctxt := list { '(obj_pair x y) : obj_tup & (var1 x y * var2 x y)%type }.
+
+    Inductive kappa_equivalence:
+      forall i o, ctxt
+      -> kappa var1 i o -> kappa var2 i o
+      -> Prop :=
+    | Var_equiv : forall i o (n1: var1 i o) (n2: var2 i o) E,
+      In (vars (obj_pair i o) (pair n1 n2)) E
+      -> kappa_equivalence E (Var n1) (Var n2)
+
+    | Abs_equiv : forall x y z 
+      (f1: var1 u x -> kappa var1 y z) 
+      (f2: var2 u x -> kappa var2 y z) 
+      (E: ctxt),
+      (forall n1 n2, kappa_equivalence (vars (obj_pair u x) (pair n1 n2) :: E) (f1 n1) (f2 n2))
+      -> kappa_equivalence E (Abs f1) (Abs f2)
+
+    | App_equiv : forall E x y z 
+      (f1 : kappa var1 (product x y) z) 
+      (f2 : kappa var2 (product x y) z) 
+      e1 e2,
+      kappa_equivalence E f1 f2
+      -> kappa_equivalence E e1 e2
+      -> kappa_equivalence E (App f1 e1) (App f2 e2)
+
+    | Compose_equiv : forall E x y z 
+      (f1: kappa var1 y z) (f2: kappa var2 y z)
+      (g1: kappa var1 x y) (g2: kappa var2 x y),
+      kappa_equivalence E f1 f2
+      -> kappa_equivalence E g1 g2
+      -> kappa_equivalence E (Comp f1 g1) (Comp f2 g2)
+
+    | Morph_equiv : forall x y E (m: morphism x y), kappa_equivalence E (Morph m) (Morph m)
+
+    | Letrec_equiv : forall x y z 
+      (v1: var1 u x -> kappa var1 u x) 
+      (v2: var2 u x -> kappa var2 u x) 
+      (f1: var1 u x -> kappa var1 y z) 
+      (f2: var2 u x -> kappa var2 y z) 
+      (E: ctxt),
+      (forall n1 n2, kappa_equivalence (vars (obj_pair u x) (pair n1 n2) :: E) (v1 n1) (v2 n2))
+      -> 
+      (forall n1 n2, kappa_equivalence (vars (obj_pair u x) (pair n1 n2) :: E) (f1 n1) (f2 n2))
+      -> 
+      kappa_equivalence E (LetRec v1 f1) (LetRec v2 f2).
+  End Equivalence.
+
+  Definition Wf {i o} (e: Kappa i o) := forall var1 var2, kappa_equivalence [] (e var1) (e var2).
+
+  Axiom Kappa_equivalence : forall {i o} (expr: forall var, kappa var i o), Wf expr.
+End Arrow.
